More Optimisations

ConditionalElimination.thy
@@ -1,7 +1,88 @@
 theory ConditionalElimination
   imports
     IREval
+    Stuttering
 begin
+
+datatype TriState = Unknown | KnownTrue | KnownFalse
+
+inductive implies :: "IRGraph \<Rightarrow> IRNode \<Rightarrow> IRNode \<Rightarrow> TriState \<Rightarrow> bool"
+  ("_ \<turnstile> _ & _ \<hookrightarrow> _") for g where
+  "g \<turnstile> (IntegerEqualsNode x y) & (IntegerLessThanNode x y) \<hookrightarrow> KnownFalse" |
+  "g \<turnstile> (IntegerEqualsNode x y) & (IntegerLessThanNode y x) \<hookrightarrow> KnownFalse" |
+
+  "g \<turnstile> x & x \<hookrightarrow> KnownTrue"
+
+inductive condition_implies :: "IRGraph \<Rightarrow> IRNode \<Rightarrow> IRNode \<Rightarrow> TriState \<Rightarrow> bool"
+  ("_ \<turnstile> _ & _ \<rightharpoonup> _") for g where
+  "\<lbrakk>\<not>(g \<turnstile> a & b \<hookrightarrow> imp)\<rbrakk> \<Longrightarrow> (g \<turnstile> a & b \<rightharpoonup> Unknown)" |
+  "\<lbrakk>(g \<turnstile> a & b \<hookrightarrow> imp)\<rbrakk> \<Longrightarrow> (g \<turnstile> a & b \<rightharpoonup> imp)"
+
+lemma implies_true_valid:
+  assumes "g \<turnstile> x & y \<rightharpoonup> imp"
+  assumes "imp = KnownTrue"
+  assumes "g m \<turnstile> x \<mapsto> v1"
+  assumes "g m \<turnstile> y \<mapsto> v2"
+  shows "v1 = v2"
+proof -
+  have "g \<turnstile> x & y \<hookrightarrow> imp"
+    using assms(1) assms(2) condition_implies.cases by blast
+then show ?thesis proof (induct x y imp rule: implies.induct)
+  case (1 x y)
+  have "imp = KnownFalse"
+    sorry
+  then show ?case
+    using assms(2) by blast
+next
+  case (2 x y)
+  have "imp = KnownFalse"
+    sorry
+  then show ?case
+    using assms(2) by blast
+next
+  case (3 x1)
+  have "x = x1 \<and> y = x1"
+    sorry
+  then have "x = y" by simp
+  then show ?case using evalDet
+    using assms(3) assms(4) by auto
+qed
+qed
+
+lemma implies_false_valid:
+  assumes "wff_graph g"
+  assumes "g \<turnstile> x & y \<rightharpoonup> imp"
+  assumes "imp = KnownFalse"
+  assumes "g m \<turnstile> x \<mapsto> v1"
+  assumes "g m \<turnstile> y \<mapsto> v2"
+  shows "v1 \<noteq> v2"
+proof -
+  have "g \<turnstile> x & y \<hookrightarrow> imp"
+    using assms(2) assms(3) condition_implies.cases by blast
+then show ?thesis proof (induct x y imp rule: implies.induct)
+  case (1 xv yv)
+  have x: "x = (IntegerEqualsNode xv yv)"
+    sorry
+  have y: "y = (IntegerLessThanNode xv yv)"
+    sorry
+  obtain xval where "g m \<turnstile> kind g xv \<mapsto> xval"
+    using assms(4) x by blast
+  obtain yval where "g m \<turnstile> kind g yv \<mapsto> yval"
+    using assms(5) y by blast
+  have "g m \<turnstile> (IntegerEqualsNode xv yv) \<mapsto> bool_to_val(xval = yval)"
+    using eval.IntegerEqualsNode
+    by (smt IntegerEqualsNodeE \<open>g m \<turnstile> kind g xv \<mapsto> xval\<close> \<open>g m \<turnstile> kind g yv \<mapsto> yval\<close> assms(4) evalDet x)
+  then show ?case
+    using eval.IntegerEqualsNode eval.IntegerLessThanNode sorry
+next
+  case (2 x y)
+  then show ?case sorry
+next
+  case (3 x1)
+  then show ?case sorry
+qed
+qed
+
 
 fun wff_stamps :: "IRGraph \<Rightarrow> bool" where
   "wff_stamps g = (\<forall> n \<in> ids g . 
@@ -13,22 +94,113 @@ lemma join_unequal:
   shows "\<nexists> x y . x = y \<and> valid_value x_stamp x \<and> valid_value y_stamp y"
   using assms disjoint_empty by auto
 
-lemma foldBinaryOpLogicJoin:
+fun replace_usages :: "ID \<Rightarrow> ID \<Rightarrow> IRGraph \<Rightarrow> IRGraph" where
+  "replace_usages nid nid' g = replace_node nid (RefNode nid', stamp g nid') g"
+
+lemma replace_usages:
+  assumes "nid \<in> ids g"
+  assumes "g' = replace_usages nid nid' g"
+  shows "kind g' nid = RefNode nid'"
+  using assms unfolding replace_usages.simps
+  using replace_node_lookup by blast
+
+lemma replace_usages_unchanged:
+  assumes "nid \<in> ids g"
+  assumes "g' = replace_usages nid nid' g"
+  shows "\<forall> n \<in> ids g . n \<noteq> nid \<longrightarrow> kind g n = kind g' n"
+  using assms unfolding replace_usages.simps
+  by (metis insertE insert_Diff replace_node_unchanged)
+
+lemma
+  assumes "(g m h \<turnstile> nid \<leadsto> nid')"
+  shows "\<forall> inter. (g \<turnstile> (nid, m, h) \<rightarrow> (inter, m, h)) \<longrightarrow> (g m h \<turnstile> nid \<leadsto> inter)"
+  using Step by auto
+
+lemma asConstantEval:
+  assumes "wff_stamps g"
+  assumes "asConstant (stamp g nid) = val"
+  assumes "val \<noteq> UndefVal"
+  assumes "g m \<turnstile> (kind g nid) \<mapsto> v"
+  shows "v = val"
+proof -
+  have "\<exists>b l h. stamp g nid = (IntegerStamp b l h)"
+    using assms(2,3) asConstant.elims by (cases "stamp g nid"; auto)
+  then obtain b l h where "stamp g nid = (IntegerStamp b l h)"
+    by blast
+  then have "l = h"
+    using asConstant.simps(1) assms(2) assms(3) by presburger
+  then have "{x . valid_value (stamp g nid) x} = {IntVal b l}"
+    using assms(2) assms(3) int_valid_range
+    using \<open>stamp g nid = IntegerStamp b l h\<close> by force
+  then show ?thesis using assms(1)
+    using \<open>l = h\<close> \<open>stamp g nid = IntegerStamp b l h\<close> assms(2) assms(4) by fastforce
+qed
+
+fun alwaysDistinct :: "Stamp \<Rightarrow> Stamp \<Rightarrow> bool" where
+  "alwaysDistinct stamp1 stamp2 = is_stamp_empty (join stamp1 stamp2)"
+
+fun neverDistinct :: "Stamp \<Rightarrow> Stamp \<Rightarrow> bool" where
+  "neverDistinct stamp1 stamp2 = (asConstant stamp1 = asConstant stamp2 \<and> asConstant stamp1 \<noteq> UndefVal)"
+
+lemma tryFoldIntegerEqualsAlwaysDistinct:
   assumes "wff_stamps g"
   assumes "kind g nid = (IntegerEqualsNode x y)"
   assumes "g m \<turnstile> (kind g nid) \<mapsto> v"
-  assumes "is_stamp_empty (join (stamp g x) (stamp g y))"
+  assumes "alwaysDistinct (stamp g x) (stamp g y)"
   shows "v = IntVal 1 0"
-  using assms eval.IntegerEqualsNode join_unequal
+  using assms eval.IntegerEqualsNode join_unequal alwaysDistinct.simps
   by (smt IntegerEqualsNodeE NoNodeE bool_to_val.simps(2) ids_some wff_stamps.simps)
 
-(*
-lemma rewriteBinaryOpLogicJoin:
+lemma tryFoldIntegerEqualsNeverDistinct:
   assumes "wff_stamps g"
-  assumes "kind g1 if = (IfNode cond t f)"
-  assumes "kind g1 cond = (IntegerEqualsNode x y)"
-  assumes "is_stamp_empty (join (stamp g x) (stamp g y))"
-  shows "?"
-*)
+  assumes "kind g nid = (IntegerEqualsNode x y)"
+  assumes "g m \<turnstile> (kind g nid) \<mapsto> v"
+  assumes "neverDistinct (stamp g x) (stamp g y)"
+  shows "v = IntVal 1 1"
+  using assms asConstantEval neverDistinct.simps
+  by (smt IntegerEqualsNodeE Value.inject(1) bool_to_val.simps(1))
+
+
+lemma replaceUsagesFoldAlwaysDistinct:
+  assumes wff: "wff_graph g \<and> wff_stamps g"
+  assumes ifkind: "kind g ifcond = (IfNode cond t f)"
+  assumes condkind: "kind g cond = (IntegerEqualsNode x y)"
+  assumes condeval: "g m \<turnstile> kind g cond \<mapsto> v"
+  assumes ran: "alwaysDistinct (stamp g x) (stamp g y)"
+  assumes g': "g' = replace_usages ifcond f g"
+  shows "\<exists>nid' .(g m h \<turnstile> ifcond \<leadsto> nid') \<longleftrightarrow> (g' m h \<turnstile> ifcond \<leadsto> nid')"
+proof -
+  have "v = IntVal 1 0"
+    using tryFoldIntegerEqualsAlwaysDistinct
+    using condeval condkind ran wff by blast
+  then have g1step: "g \<turnstile> (ifcond, m, h) \<rightarrow> (f, m, h)"
+    by (metis IfNode condeval ifkind val_to_bool.simps(1))
+  have g2step: "g' \<turnstile> (ifcond, m, h) \<rightarrow> (f, m, h)"
+    using g' unfolding replace_usages.simps
+    by (simp add: step.RefNode)
+  from g1step g2step show ?thesis
+    using Step by blast
+qed
+
+lemma replaceUsagesFoldNeverDistinct:
+  assumes wff: "wff_graph g \<and> wff_stamps g"
+  assumes ifkind: "kind g ifcond = (IfNode cond t f)"
+  assumes condkind: "kind g cond = (IntegerEqualsNode x y)"
+  assumes condeval: "g m \<turnstile> kind g cond \<mapsto> v"
+  assumes ran: "neverDistinct (stamp g x) (stamp g y)"
+  assumes g': "g' = replace_usages ifcond t g"
+  shows "\<exists>nid' .(g m h \<turnstile> ifcond \<leadsto> nid') \<longleftrightarrow> (g' m h \<turnstile> ifcond \<leadsto> nid')"
+proof -
+  have "v = IntVal 1 1"
+    using tryFoldIntegerEqualsNeverDistinct
+    using condeval condkind ran wff by blast
+  then have g1step: "g \<turnstile> (ifcond, m, h) \<rightarrow> (t, m, h)"
+    by (smt IfNode condeval ifkind val_to_bool.simps(1))
+  have g2step: "g' \<turnstile> (ifcond, m, h) \<rightarrow> (t, m, h)"
+    using g' unfolding replace_usages.simps
+    by (simp add: step.RefNode)
+  from g1step g2step show ?thesis
+    using Step by blast
+qed
 
 end
