Stuttering.thy
@@ -1,0 +1,26 @@
+theory Stuttering
+imports IRStepObj
+begin
+
+inductive stutter:: "IRGraph \<Rightarrow> MapState \<Rightarrow> DynamicHeap \<Rightarrow> ID \<Rightarrow> ID \<Rightarrow> bool" ("_ _ _ \<turnstile> _ \<leadsto> _" 55)
+  for g m h where
+
+  Step:
+  "\<lbrakk>g \<turnstile> (nid,m,h) \<rightarrow> (nid',m,h)\<rbrakk>
+   \<Longrightarrow> g m h \<turnstile> nid \<leadsto> nid'" |
+
+  Transitive:
+  "\<lbrakk>g \<turnstile> (nid,m,h) \<rightarrow> (nid'',m,h);
+    g m h \<turnstile> nid'' \<leadsto> nid'\<rbrakk>
+   \<Longrightarrow> g m h \<turnstile> nid \<leadsto> nid'"
+
+text_raw \<open>\Snip{Stutter}%\<close>
+text \<open>
+\begin{center}
+@{thm[mode=Rule] stutter.Step [no_vars]}\\[8px]
+@{thm[mode=Rule] stutter.Transitive [no_vars]}
+\end{center}
+\<close>
+text_raw \<open>\EndSnip\<close>
+
+end
